examples/HolOmega/interim/KmonadScript.sml
@@ -7,8 +7,14 @@ open HolKernel Parse boolLib
      bossLib
 
 open combinTheory pairTheory categoryTheory ;
+open auxLib ;
 (*
+load "auxLib" ;
 load "KmonadTheory" ; open KmonadTheory ;
+fun sge tm = set_goal ([], tm) ;
+fun eev tacs = e (EVERY tacs) ;
+fun eall [] = () 
+  | eall (t :: ts) = (e t ; eall ts) ;
 *)
 
 val _ = set_trace "Unicode" 1;
@@ -28,8 +34,8 @@ val Kcomp_def = new_definition("Kcomp_def", Term
      comp (ext h) k : ('A,'M,'a,'c) Kleisli`) ;
 
 val Kmonad_def = new_definition("Kmonad_def", Term
-   `Kmonad ((id, comp) : 'A category) 
-     (unit: (!'a. ('a, 'a 'M) 'A), ext: 'M ('A ext)) = 
+   `Kmonad = \:'A 'M. \ ((id, comp) : 'A category) 
+     (unit: (!'a. ('a, 'a 'M) 'A), ext: 'M ('A ext)). 
       (* Left unit *)
           (!:'a 'b. !(k: ('a, 'b 'M) 'A). comp (ext k) unit = k) /\
       (* Right unit *)
@@ -38,8 +44,22 @@ val Kmonad_def = new_definition("Kmonad_def", Term
           (!:'a 'b 'c. !(k:('a, 'b 'M) 'A) (h:('b, 'c 'M) 'A).
 	      comp (ext h) (ext k) = ext (comp (ext h) k))`);
 
-val (Kcat_monadD, _) = EQ_IMP_RULE (SPEC_ALL Kmonad_def) ;
-val [KcmRU, KcmLU, KcmAss] = CONJUNCTS (UNDISCH Kcat_monadD) ;
+val Kmonad_thm = store_thm ("Kmonad_thm", Term
+   `Kmonad ((id, comp) : 'A category) 
+     (unit: (!'a. ('a, 'a 'M) 'A), ext: 'M ('A ext)) = 
+      (* Left unit *)
+          (!:'a 'b. !(k: ('a, 'b 'M) 'A). comp (ext k) unit = k) /\
+      (* Right unit *)
+          (!:'a.  ext (unit : ('a, 'a 'M) 'A) = id) /\
+      (* Associative *)
+          (!:'a 'b 'c. !(k:('a, 'b 'M) 'A) (h:('b, 'c 'M) 'A).
+	      comp (ext h) (ext k) = ext (comp (ext h) k))`,
+  SRW_TAC [] [Kmonad_def]) ;
+
+val (KmonadD, _) = EQ_IMP_RULE (SPEC_ALL Kmonad_thm) ;
+val [KmonDRU, KmonDLU, KmonDAss] = map DISCH_ALL (CONJUNCTS (UNDISCH KmonadD)) ;
+val _ = map save_thm [("KmonDLU", KmonDLU), ("KmonDRU", KmonDRU),
+  ("KmonDAss", KmonDAss)] ;
 
 (* Kleisli category is a category iff 'M is a monad *)
 
@@ -50,7 +70,7 @@ val Kcat_IMP_Kmonad = store_thm ("Kcat_IMP_Kmonad",
   ``category [:'A:] (id, comp) /\
     category [: ('A, 'M) Kleisli :] (unit, Kcomp (id, comp) ext) ==>
     Kmonad (id, comp) (unit, ext : ('A, 'M) ext)``,
-    (REWRITE_TAC [Kmonad_def, Kcomp_def]) THEN
+    (REWRITE_TAC [Kmonad_thm, Kcomp_def]) THEN
     (REPEAT STRIP_TAC) THENL [
     EVERY [
       (POP_ASSUM (ASSUME_TAC o MATCH_MP catDRU)),
@@ -76,7 +96,6 @@ val Kcat_IMP_Kmonad = store_thm ("Kcat_IMP_Kmonad",
       (FIRST_ASSUM (ASSUME_TAC o MATCH_MP catDRU)),
       (ASM_REWRITE_TAC []) ]]) ;
 
-
 (* this next doesn't work (doesn't parse properly) without the type 
   parameter for category (even with a type annotation, ie
   category ((unit, Kcomp (id, comp) ext) : ('A, 'M) Kleisli category)
@@ -86,7 +105,7 @@ val Kmonad_IMP_Kcat = store_thm ("Kmonad_IMP_Kcat",
   ``category [:'A:] (id, comp) /\
     Kmonad (id, comp) (unit, ext : ('A, 'M) ext) ==> 
     category [: ('A, 'M) Kleisli :] (unit, Kcomp (id, comp) ext)``,
-  EVERY [ (REWRITE_TAC [category_def, Kmonad_def, Kcomp_def]),
+  EVERY [ (REWRITE_TAC [category_def, Kmonad_thm, Kcomp_def]),
     (CONV_TAC (DEPTH_CONV TY_BETA_CONV)),
     (REWRITE_TAC [o_THM, I_THM, FUN_EQ_THM, UNCURRY_DEF]),
     (CONV_TAC (TOP_DEPTH_CONV (BETA_CONV ORELSEC TY_BETA_CONV))),
@@ -150,7 +169,7 @@ val Kmonad_IMP_uof = store_thm ("Kmonad_IMP_uof",
   ``category [:'A:] (id,comp) /\ Kmonad (id,comp) (unit,ext) ==>
     g_functor [:'A, ('A, 'M) Kleisli :] (id, comp) 
       (unit, Kcomp (id,comp) ext) (\:'a 'b. comp [:'a,'b,'b 'M:] unit)``,
-  EVERY [ (REWRITE_TAC [Kmonad_def, Kcomp_def, g_functor_thm, category_thm]),
+  EVERY [ (REWRITE_TAC [Kmonad_thm, Kcomp_def, g_functor_thm, category_thm]),
     STRIP_TAC, TY_BETA_TAC, BETA_TAC, (ASM_REWRITE_TAC []) ]) ;
     
 (*
@@ -161,11 +180,10 @@ set_goal ([], it) ;
 val (sgs, goal) = top_goal () ;
 *)
 
-    
 val Kmonad_IMP_ext_f = store_thm ("Kmonad_IMP_ext_f",
   ``Kmonad (id,comp) (unit,ext) ==> g_functor [: ('A, 'M) Kleisli, 'A :] 
       (unit, Kcomp (id,comp) ext) (id, comp) ext``,
-  EVERY [ (REWRITE_TAC [Kmonad_def, Kcomp_def, g_functor_thm]),
+  EVERY [ (REWRITE_TAC [Kmonad_thm, Kcomp_def, g_functor_thm]),
     STRIP_TAC, (CONJ_TAC THEN1 FIRST_ASSUM ACCEPT_TAC),
     TY_BETA_TAC, BETA_TAC, (CONV_TAC (ONCE_DEPTH_CONV SYM_CONV)),
     (FIRST_ASSUM ACCEPT_TAC) ]) ;
@@ -174,9 +192,148 @@ val Kmonad_IMP_unit_nt = store_thm ("Kmonad_IMP_unit_nt",
   ``Kmonad (id,comp) (unit,ext) ==> 
     g_nattransf [:'A:] (id, comp) unit (g_I [:'A:]) 
       (\: 'a 'b. \f. ext [:'a,'b:] (comp (unit [:'b:]) f))``,
-  EVERY [ (REWRITE_TAC [Kmonad_def, Kcomp_def, g_I_def, g_nattransf_thm]),
+  EVERY [ (REWRITE_TAC [Kmonad_thm, Kcomp_def, g_I_def, g_nattransf_thm]),
     STRIP_TAC, TY_BETA_TAC, BETA_TAC, (ASM_REWRITE_TAC [I_THM]) ]) ;
 
+val Kmonad_extomap' = prove (
+  ``category [:'A:] (id, comp) /\ Kmonad [:'A,'M:] (id,comp) (unit,ext) ==> 
+    (ext (comp g f) = comp (ext g) (ext (comp unit f)))``,
+  EVERY [ (REWRITE_TAC [Kmonad_thm, Kcomp_def, category_thm]),
+    STRIP_TAC, (ASM_REWRITE_TAC []) ]) ;
+
+val Kmonad_extomap = save_thm ("Kmonad_extomap", 
+  (DISCH_ALL o TY_GEN_ALL o GEN_ALL o UNDISCH_ALL) Kmonad_extomap') ;
+
+(* approach to distributive law for monads;
+  a monad in the Kleisli category of another monad *)
+(* first note this type equality *)
+val true = Type `: (('A, 'M) Kleisli, 'N) Kleisli` =
+  Type `: ('A, 'N o 'M) Kleisli` ;
+
+(* following fails typechecking when both monad type arguments 
+  ('N and 'N o 'M) are deleted *)
+val tmpext = ``category (id, comp) /\ 
+  Kmonad [:'A:] (id,comp) (unitM, extM : ('A, 'M) ext) /\ 
+  Kmonad [: ('A, 'M) Kleisli, 'N :] 
+    (unitM, Kcomp (id,comp) extM) (unitNM, pext) ==>
+  Kmonad [: 'A, 'N o 'M :] (id, comp) (unitNM, \:'a 'b. extM o pext)`` ;
+
+val pext_cm = store_thm ("pext_cm", tmpext,
+  EVERY [ STRIP_TAC,
+    (MATCH_MP_TAC Kcat_IMP_Kmonad),
+    (ASM_REWRITE_TAC [Kcomp_def]), TY_BETA_TAC,
+    (IMP_RES_TAC Kmonad_IMP_Kcat),
+    (POP_ASSUM_LIST (MAP_EVERY (ASSUME_TAC o CONV_RULE (REDEPTH_CONV
+      (REWR_CONV Kcomp_def ORELSEC TY_BETA_CONV ORELSEC BETA_CONV))))),
+    (ASM_REWRITE_TAC [combinTheory.o_THM]) ]) ;
+
+val EQ_IMP_IMP =
+  auxLib.sfg (auxLib.ufd CONJUNCT1 o fst o EQ_IMP_RULE) EQ_IMP_THM ;
+val hrk = (hd (RES_CANON Kmonad_extomap)) ;
+
+val tmepe = ``category (id, comp) /\ 
+  Kmonad [:'A:] (id,comp) (unitM, extM : ('A, 'M) ext) /\ 
+  (!: 'a 'b. !f : ('a, 'b 'N 'M) 'A. 
+    extM ((extNM : ('A, 'N o 'M) ext) f) = comp (extNM f) (extM id)) /\
+  (pext = \:'a 'b. \f. comp (extNM f) unitM) ==>
+  (!: 'a 'b. !f : ('a, 'b 'N 'M) 'A. extM (pext f) = extNM f)`` ;
+
+val J1_IMP_ext_pext = store_thm ("J1_IMP_ext_pext", tmepe,
+  EVERY [ STRIP_TAC, (ASM_REWRITE_TAC []), 
+    (REPEAT STRIP_TAC), TY_BETA_TAC, BETA_TAC,
+    (FIRST_ASSUM (fn th => 
+      let val mat1 = MATCH_MP hrk th 
+      in FIRST_ASSUM (fn ath => 
+          (ONCE_REWRITE_TAC [MATCH_MP mat1 ath])) end)),
+    (ASM_REWRITE_TAC []), 
+    (FIRST_ASSUM (fn th => 
+      (REWRITE_TAC [GSYM (MATCH_MP catDAss th)]))),
+    (FIRST_ASSUM (fn th => 
+      let val mat1 = MATCH_MP hrk th 
+      in FIRST_ASSUM (fn ath => 
+          (ONCE_REWRITE_TAC [GSYM (MATCH_MP mat1 ath)])) end)),
+    (FIRST_ASSUM (fn th => (REWRITE_TAC [MATCH_MP catDLU th]))),
+    (FIRST_X_ASSUM (fn th => (REWRITE_TAC [MATCH_MP KmonDLU th]))),
+    (FIRST_X_ASSUM (fn th => (REWRITE_TAC [MATCH_MP catDRU th]))) ]) ;
+
+val tmpexti = ``category (id, comp) /\ 
+  Kmonad [:'A:] (id,comp) (unitM, extM : ('A, 'M) ext) /\ 
+  Kmonad [: 'A, 'N o 'M :] (id, comp) (unitNM, extNM) /\
+  (!: 'a 'b. !f : ('a, 'b 'N 'M) 'A. 
+    extM (extNM f) = comp (extNM f) (extM id)) /\
+  (pext = \:'a 'b. \f. comp (extNM f) unitM) ==>
+  Kmonad [: ('A, 'M) Kleisli, 'N :] 
+    (unitM, Kcomp (id,comp) extM) (unitNM, pext)`` ;
+
+(* can't do MATCH_MP_TAC (GSYM J1_IMP_ext_pext) ; *)
+val gjs = (DISCH_ALL o GSYM o SPEC_ALL o TY_SPEC_ALL o UNDISCH)
+  J1_IMP_ext_pext ;
+
+val cm_if_J1 = store_thm ("cm_if_J1", tmpexti,  
+  EVERY [ STRIP_TAC,
+    (MATCH_MP_TAC Kcat_IMP_Kmonad),
+    (IMP_RES_TAC Kmonad_IMP_Kcat),
+    (FIRST_X_ASSUM (fn th => CONJ_TAC THEN1 ACCEPT_TAC th)),
+    (FIRST_X_ASSUM (fn th => EVERY [MP_TAC th, MATCH_MP_TAC EQ_IMP_IMP,
+      BETA_TY_TAC, AP_TERM_TAC, AP_TERM_TAC])),
+    (REWRITE_TAC [Kcomp_def, FUN_EQ_THM, TY_FUN_EQ_THM]),
+    (* need tactic for \x. A = \y. A *)
+    (REPEAT STRIP_TAC), TY_BETA_TAC, BETA_TAC,
+    AP_THM_TAC, AP_TERM_TAC, (MATCH_MP_TAC gjs),
+    (ASM_REWRITE_TAC []) ]) ;
+
+(* equivalence between compound monads arising from a monad in the 
+  Kleisli category of another monad, and compound monads satisfying
+  Jones & Duponcheel condition J1 *)
+val tm_Kc_J1 = 
+  ``category (id,comp) /\ Kmonad (id,comp) (unitM,extM) ==> 
+  (Kmonad [: 'A, 'N o 'M :] (id,comp) (unitNM,extNM) /\
+  (!: 'a 'b. !f : ('a, 'b 'N 'M) 'A. 
+    extM [:'a 'N 'M, 'b 'N:] (extNM f) = 
+      comp (extNM f) (extM [:'a 'N 'M, 'a 'N:] id)) /\
+  (pext = (\:'a 'b. (\f. comp (extNM f) unitM))) = 
+  Kmonad [:('A,'M) Kleisli, 'N:] (unitM,Kcomp (id,comp) extM) (unitNM,pext) /\
+  (extNM = (\:'a 'b. (\f. extM (pext f)))))`` ;
+
+val cm_Kc_J1 = store_thm ("cm_Kc_J1", tm_Kc_J1, 
+  EVERY [STRIP_TAC, EQ_TAC, REPEAT STRIP_TAC, REPEAT CONJ_TAC]
+  THENL [
+    (MATCH_MP_TAC cm_if_J1 THEN ASM_REWRITE_TAC []),
+    EVERY [ 
+      (REWRITE_TAC [FUN_EQ_THM, TY_FUN_EQ_THM]),
+      (REPEAT STRIP_TAC), TY_BETA_TAC, BETA_TAC,
+      MATCH_MP_TAC gjs, (ASM_REWRITE_TAC []) ],
+
+    EVERY [ (MP_TAC pext_cm),
+      (ASM_REWRITE_TAC []),
+      (MATCH_MP_TAC EQ_IMP_IMP),
+      (REPEAT (AP_THM_TAC ORELSE AP_TERM_TAC)),
+      (REWRITE_TAC [FUN_EQ_THM, TY_FUN_EQ_THM]),
+      (REPEAT STRIP_TAC), TY_BETA_TAC, BETA_TAC,
+      (MATCH_ACCEPT_TAC combinTheory.o_THM) ],
+
+    EVERY [
+      (ASM_REWRITE_TAC []), TY_BETA_TAC, BETA_TAC,
+      (FIRST_X_ASSUM (fn th => 
+	CHANGED_TAC (REWRITE_TAC [(MATCH_MP KmonDAss th)]))),
+      (FIRST_X_ASSUM (fn th => 
+	(REWRITE_TAC [(MATCH_MP catDRU th)]))) ],
+
+    EVERY [
+      (ASM_REWRITE_TAC []), TY_BETA_TAC, BETA_TAC, 
+      (IMP_RES_TAC KmonDRU),
+      (ASM_REWRITE_TAC []),
+      (CONV_TAC (DEPTH_CONV ETA_CONV)), 
+      (CONV_TAC (DEPTH_CONV TY_ETA_CONV)), 
+      REFL_TAC ] ]) ;
+
+(*
+show_types := true ;
+show_types := false ;
+handle e => Raise e ;
+set_goal ([], it) ;
+val (sgs, goal) = top_goal () ;
+*)
 
 val _ = set_trace "types" 1;
 val _ = set_trace "kinds" 0;
